# 1. Let f be a group homomorphism from G to H. Let L be a subgroup of Im(f ). Show that $f^{−1}(L)/ \ker f \cong L$
$f: G \rightarrow H$, $L \leq \operatorname{Im} f \subset H$

Solution

Let $\tilde{f}: f^{-1}(L) \rightarrow L$, $\tilde{f}(g) = f(g)$.

First, $f^{-1}(L)\leq G$, since $\forall g_1, g_2 \in f^{-1}(L)$, $f(g_1 g_2^{-1}) = f(g_1)f(g_2)^{-1} \in L$

Then obviously $\tilde{f}$ is surjective and homomorphism

Also, $\ker \tilde{f} = \ker f$, since $0 \in L \cap \operatorname{Im}  f$, and that $\tilde{f}(g) = 0 \Leftrightarrow f(g) = 0$

So by the first isomorphism theorem, we have $f^{-1}(L)/ \ker f \cong L$

# 2. Let A, B be two subsets of a finite group G. If A + B > G, show thatG = AB

Solution

Since $A, B \subset G$, by closure trivially we have $AB \subset G$

For $G \subset AB$, $\forall g \in G$, consider all element in $A^{-1}g$, which is all the element resulting in $g$ after a right multiplication with A. Here $A^{-1} = \{a^{-1} | a \in A\}$

Since
$$
|A| = |A^{-1}| = |A^{-1}g|
$$
$$
|A^{-1}g|  + |B| > |G|
$$

we have $A^{-1}g \cap B \neq \emptyset$. So $\exists a \in A, b \in B$, such that $a^{-1}g = b$, $ab = aa^{-1}g = g \in AB$

So $G \subset AB$, $G = AB$

# 3. The Fourth Isomorphism Theorem
Let $H ◁ G$. Define $A= \{M : H ≤M, M ≤G\}$,  $\bar A$ = set of subgroups of $G/H$. Show that there is a bijection between $A$ and $\bar A$. Furthermore, show that $M ◁ G ⇐⇒(M/H) ◁ (G/H)$
===

Solution

Let $\phi: A \rightarrow \bar A$, $\phi(M) = M/H$

surjective:  

$\forall S \leq G/H$, let $M \triangleq \{g \in G \mid gH \in S\}$.
- $M \leq G$, since $\forall g_1, g_2 \in M$, $g_1H, g_2H \in S$, $g_1(g_2)^{-1}H \in S$, so $g_1g_2^{-1} \in M$
- $H\leq M$, since $\forall h\in H, hH = H  \in S$, $H \subset M$.
- So $M \in A$, $H\triangleleft M$, and $\phi(M) = S$

injective:

$\forall M_1, M_2 \in A$ such that $M_1/H = M_2/H$. $\forall m_1\in M$,

$\exist m_2 \in M_2$ such that $m_1H = m_2H$, so $m_2^{-1}m_1 \in H \subset M_2$, so $m_1 = m_2m_2^{-1}m_1 \in M_2$, $M_1 \subset M_2$

Similarly, $M_2 \subset M_1$, so $M_1 = M_2$

So $\phi$ is a bijection.

Furthermore, 

Suppose $M \triangleleft G$, then $(gH)(M/H)(gH)^{-1} = (gMg^{-1})/H = M/H$. wo $M/H \triangleleft G/H$

Suppose $M/H \triangleleft G/H$, consider $\sigma: \sigma(g) = (gH)(M/H)$, which is a homomorphism composition by $G \rightarrow G/H$ and $G/H \rightarrow G/H/ M/H$. The kernel of $\sigma$ is $\{g\in G\mid gH(M/H) = M/H\} = \{g\in G \mid gH \in M/H\} = \{g \in G\mid g\in M\} = M$, so
$$M = \ker \sigma \triangleleft G$$

# 4. Show that the given two groups are isomorphic.
## (a)
$(\Reals/\Z, +) \cong (S = \{e^{j\theta}, \theta \in [0,2\pi)\}, *)$

Let $\phi: \Reals \rightarrow S$, $\phi(x) = e^{j2\pi x}$, this is homomorphism since $\phi(x+y) = e^{2\pi j(x+y) }=\phi(x)\phi(y)$
- $\operatorname{Im} \phi = S$
- $\ker \phi = \{x \in \Reals\mid 2\pi x = 2k\pi, k\in Z\}= \Z$

By the first isomorphism theorem, $\Reals/\Z \cong S$

## (b)
$C^*/\Reals_{>0} \cong (S, *)$

Let $\phi: C^* \rightarrow S$, $\phi(z) = \frac{z}{|z|}$; this is homomorphism since  $\phi(z_1z_2) = \frac{z_1z_2}{|z_1z_2|} = \frac{z_1}{|z_1|}\frac{z_2}{|z_2|} = \phi(z_1)\phi(z_2)$

- $\operatorname{Im} \phi = S$
- $\ker\phi = \{z \in C^* \mid \frac{z}{|z|} = 1\} = \Reals_{>0}$

By the first isomorphism theorem, $C^*/\Reals_{>0} \cong S$

## (c)
$C^*/R^* \cong S$

Let $\phi: C^* \rightarrow S$, $\phi(z) = \left(\frac{z}{|z|}\right)^2$; this is homomorphism since $\phi(z_1z_2) = \left(\frac{z_1z_2}{|z_1z_2|}\right)^2 = \left(\frac{z_1}{|z_1|}\right)^2\left(\frac{z_2}{|z_2|}\right)^2 = \phi(z_1)\phi(z_2)$

- $\operatorname{Im} \phi = S$
- $\ker\phi = \{z \in C^* \mid 2\theta \in \{0, 2\pi\}, z = re^{j\theta}\} = R^*$

By the first isomorphism theorem, $C^*/R^* \cong S$

# 5. If $σ = (i_1i_2 \cdots i_t) ∈S_n$, show that $∀τ ∈S_n$, $τ στ^{−1} = (τ (i1)τ (i2) ···τ (it))$

Equivalently, show that $\tau \sigma = (\tau (i_1)\tau (i_2)\cdots\tau (i_t))\tau$

$\forall j\leq t$, consider $i_j$ affected by $\sigma$,
$$
(\tau \sigma)(i_j) = \tau(\sigma(i_j)) = \tau(i_{j+1})
$$
$$
((\tau (i_1)\tau (i_2)\cdots\tau (i_t))\circ \tau)(i_j) = (\tau (i_1)\tau (i_2)\cdots\tau (i_t))\tau(i_j) = \tau(i_{j+1})
$$

The rest of element is not affected.

So $\tau \sigma = (\tau (i_1)\tau (i_2)\cdots\tau (i_t))\tau$

# 6. Show that $S_n$ is generated by σ = (12) and τ = (12 ···n)
By `homework 5`, $\sigma \tau \sigma^{-1} = (23)$. Similarly, $\sigma^k \tau \sigma^{-k} = (k+1, k+2)$

Also, $(23)(12)(23)^{-1} = (1,3)$, similarly, $(k-1, k)(1,k-1)(k-1, k)^{-1} = (1, k)$

Note that $(i,j)= (1, i)(1,j)(1,i)^{-1}$

So every transposition can be generated by $\sigma$ and $\tau$, and every permutation can be generated by transposition.

# 7. Show that N = {(1), (12)(34), (13)(24), (14)(23)} is a normal subgroup of $S_4$. Furthermore, show that $S_4/N ≃S_3$ and $A_4/N ≃Z_3$
$N\leq S_4$.

1. Closure: $(1j)(kl)\circ (1k)(jl) = (1l)(jk) \in N$, similar for $(1j)(kl)\circ (1l)(jk)$
2. Identity: $(1) \in N$
3. Inverse: $\forall n \in N$, $n^2 = (1)$. $n^{-1} = n$

$N \triangleleft S_4$.

- $\forall \sigma=(ab)(cd) \in S_4$, by HW 5, $s\sigma s^{-1} = s(ab)s^{-1}s(cd)s^{-1} =(s(a)s(b))(s(c)s(d)) \in N$
- For identity, $s(1)s^{-1} = (1) \in N$

$S_4/N \cong S_3$

The cosets are 
$$
N, (123)N = \{(123),(134),(324),(142)\}
$$
$$
(132)N = \{(132),(234),(124),(143)\},
(12)N = \{(12),(34),(1324),(1423)\}
$$
$$(13)N = \{(13),(1234),(24),(1432)\},
(23)N = \{(23),(1342),(1243),(14)\}
$$

Note that the representitive of the cosets are $(1), (123), (132), (12), (13), (23)$, which is $S_3$. 

Let $\phi: S_3 \rightarrow S_4/N$, $\phi(\sigma) = \sigma' N$, where $\sigma'$ used in RHS is the one in $S_4$ that have the same writing pattern as the $\sigma$ in LHS. This is clearly a bijection. And it is homomorphism since the written pattern is preserved under multiplication.

$A_4/N \cong Z_3$

Note that $|A_4| = 12$, $|N| = 4$, so $|A_4/N| = 3$. It must be cyclic. So
$$
A_4/N \cong Z_3
$$




# 8. Show that A4 has no subgroup of order 6.
$|A_4| = 4!/2 = 12$, suppose it has a subgroup $H$ of order 6, then $[A_4 :H] = 2$. Then $A_4$ can be disjointly written as $A_4 = H \cup xH$

Let $x$ be a $3$-cycle, $x\notin H$. Consider the cosets $H, xH, x^2H$. Since $[A_4: H] = 2$, two of the cosets must be equal. But $H$ and $xH$ are distinct, so $x^2H$ must be equal to one of them.

If $x^2H = H$, then $x^2 \in H$, so $x^{-1} \in H$, contradiction.

If $x^2H = xH$, then $x^2 \in xH$, so $x \in H$, contradiction.

So $A_4$ has no subgroup of order 6.